Variants: DSBA Group 211
---

1. Variant
```
f0(a, b, c, d) = MAX(a, b, c, d)
f1(x) = -6*x^3 + 8*x^2 + 8*x + 4
f2(x) = sin(4*x)*9 + 9
f3(x) = (-3)^x + 8
f4(x) = 1 / (1 + e^(5*x))
```
2. Variant
```
f0(a, b, c, d) = MAX(a, b, c, d)
f1(x) = 5*x^3 + 9*x^2 - 6*x + 2
f2(x) = sin(-3*x)*3 + 6
f3(x) = 4^x - 9
f4(x) = 1 / (1 + e^(-1*x))
```
3. Variant
```
f0(a, b, c, d) = L2(a, b, c, d) = sqrt(a^2 + b^2 + c^2 + d^2)
f1(x) = 2*x^3 + 7*x^2 + 3*x + 2
f2(x) = sin(-2*x)*3 - 7
f3(x) = (-4)^x + 3
f4(x) = 1 / (1 + e^(8*x))
```
4. Variant
```
f0(a, b, c, d) = AVG(a, b, c, d) = (a + b + c + d) / 4
f1(x) = 6*x^3 + 6*x^2 - 4*x + 8
f2(x) = sin(-8*x)*2 - 6
f3(x) = (-2)^x - 1
f4(x) = 1 / (1 + e^(3*x))
```
5. Variant
```
f0(a, b, c, d) = AVG(a, b, c, d) = (a + b + c + d) / 4
f1(x) = -6*x^3 - 2*x^2 + 2*x + 2
f2(x) = sin(-8*x)*(-5) + 6
f3(x) = (-9)^x + 7
f4(x) = 1 / (1 + e^(-7*x))
```
6. Variant
```
f0(a, b, c, d) = AVG(a, b, c, d) = (a + b + c + d) / 4
f1(x) = -7*x^3 + 8*x^2 + 3*x - 7
f2(x) = sin(7*x)*3 + 6
f3(x) = (-9)^x - 1
f4(x) = 1 / (1 + e^(8*x))
```
7. Variant
```
f0(a, b, c, d) = L2(a, b, c, d) = sqrt(a^2 + b^2 + c^2 + d^2)
f1(x) = -5*x^3 - 6*x^2 - 2*x + 6
f2(x) = sin(-6*x)*(-7) - 1
f3(x) = (-7)^x + 5
f4(x) = 1 / (1 + e^(5*x))
```
8. Variant
```
f0(a, b, c, d) = L2(a, b, c, d) = sqrt(a^2 + b^2 + c^2 + d^2)
f1(x) = -2*x^3 - 1*x^2 + 6*x + 9
f2(x) = sin(9*x)*(-2) + 8
f3(x) = 5^x + 2
f4(x) = 1 / (1 + e^(-3*x))
```
9. Variant
```
f0(a, b, c, d) = MIN(a, b, c, d)
f1(x) = -8*x^3 + 2*x^2 - 2*x - 3
f2(x) = sin(3*x)*(-9) + 7
f3(x) = (-8)^x - 9
f4(x) = 1 / (1 + e^(2*x))
```
10. Variant
```
f0(a, b, c, d) = L2(a, b, c, d) = sqrt(a^2 + b^2 + c^2 + d^2)
f1(x) = -5*x^3 - 5*x^2 + 5*x - 7
f2(x) = sin(6*x)*(-1) - 5
f3(x) = 9^x - 7
f4(x) = 1 / (1 + e^(1*x))
```
11. Variant
```
f0(a, b, c, d) = L2(a, b, c, d) = sqrt(a^2 + b^2 + c^2 + d^2)
f1(x) = 6*x^3 + 8*x^2 - 5*x + 1
f2(x) = sin(-9*x)*9 - 7
f3(x) = (-2)^x - 1
f4(x) = 1 / (1 + e^(-1*x))
```
12. Variant
```
f0(a, b, c, d) = MAX(a, b, c, d)
f1(x) = 2*x^3 + 8*x^2 + 7*x - 6
f2(x) = sin(-6*x)*6 - 5
f3(x) = 3^x + 9
f4(x) = 1 / (1 + e^(5*x))
```
13. Variant
```
f0(a, b, c, d) = MIN(a, b, c, d)
f1(x) = 6*x^3 + 6*x^2 - 3*x - 3
f2(x) = sin(2*x)*7 - 1
f3(x) = 2^x + 4
f4(x) = 1 / (1 + e^(-1*x))
```
14. Variant
```
f0(a, b, c, d) = L2(a, b, c, d) = sqrt(a^2 + b^2 + c^2 + d^2)
f1(x) = 8*x^3 - 2*x^2 - 2*x - 3
f2(x) = sin(-7*x)*2 + 4
f3(x) = (-5)^x - 2
f4(x) = 1 / (1 + e^(7*x))
```
15. Variant
```
f0(a, b, c, d) = MAX(a, b, c, d)
f1(x) = 5*x^3 + 4*x^2 + 2*x - 4
f2(x) = sin(-4*x)*(-3) + 5
f3(x) = 6^x - 8
f4(x) = 1 / (1 + e^(-5*x))
```
16. Variant
```
f0(a, b, c, d) = AVG(a, b, c, d) = (a + b + c + d) / 4
f1(x) = -3*x^3 + 8*x^2 + 8*x + 3
f2(x) = sin(-6*x)*7 + 3
f3(x) = (-3)^x - 3
f4(x) = 1 / (1 + e^(4*x))
```
17. Variant
```
f0(a, b, c, d) = L2(a, b, c, d) = sqrt(a^2 + b^2 + c^2 + d^2)
f1(x) = 7*x^3 + 8*x^2 - 1*x - 9
f2(x) = sin(-5*x)*9 + 7
f3(x) = (-4)^x + 5
f4(x) = 1 / (1 + e^(7*x))
```
18. Variant
```
f0(a, b, c, d) = MAX(a, b, c, d)
f1(x) = 1*x^3 + 5*x^2 - 9*x - 8
f2(x) = sin(-5*x)*(-8) + 7
f3(x) = 2^x + 2
f4(x) = 1 / (1 + e^(5*x))
```
19. Variant
```
f0(a, b, c, d) = AVG(a, b, c, d) = (a + b + c + d) / 4
f1(x) = 2*x^3 - 2*x^2 + 8*x - 3
f2(x) = sin(5*x)*2 + 8
f3(x) = 9^x - 5
f4(x) = 1 / (1 + e^(9*x))
```
20. Variant
```
f0(a, b, c, d) = AVG(a, b, c, d) = (a + b + c + d) / 4
f1(x) = 4*x^3 + 6*x^2 + 9*x - 7
f2(x) = sin(-7*x)*(-4) + 2
f3(x) = (-5)^x - 9
f4(x) = 1 / (1 + e^(7*x))
```
21. Variant
```
f0(a, b, c, d) = L2(a, b, c, d) = sqrt(a^2 + b^2 + c^2 + d^2)
f1(x) = -2*x^3 + 8*x^2 - 6*x + 9
f2(x) = sin(-5*x)*2 + 2
f3(x) = (-8)^x - 9
f4(x) = 1 / (1 + e^(1*x))
```
22. Variant
```
f0(a, b, c, d) = MAX(a, b, c, d)
f1(x) = -3*x^3 + 7*x^2 - 3*x + 4
f2(x) = sin(8*x)*(-8) - 2
f3(x) = (-6)^x - 6
f4(x) = 1 / (1 + e^(3*x))
```
23. Variant
```
f0(a, b, c, d) = MIN(a, b, c, d)
f1(x) = -2*x^3 + 1*x^2 + 8*x - 8
f2(x) = sin(9*x)*5 - 4
f3(x) = (-7)^x + 2
f4(x) = 1 / (1 + e^(2*x))
```
24. Variant
```
f0(a, b, c, d) = AVG(a, b, c, d) = (a + b + c + d) / 4
f1(x) = 7*x^3 - 1*x^2 + 9*x - 3
f2(x) = sin(3*x)*(-2) + 5
f3(x) = (-6)^x + 2
f4(x) = 1 / (1 + e^(-5*x))
```
---
